ulib/FStar.Ghost.fsti
@@ -58,6 +58,31 @@ val hide_reveal (#a: Type) (x: erased a)
 
 val reveal_hide (#a: Type) (x: a) : Lemma (ensures (reveal (hide x) == x)) [SMTPat (hide x)]
 
+(* We use Spec as a more descriptive abbreviation for GTot
+     - They are specificational, i.e., Spec in the sense of specification
+     - They are also ghostly, i.e, Spec in the sense of Specter
+   *)
+effect Spec (a:Type) = GTot a
+
+(* pull is an axiom.
+
+   It can be given a model in some implementations of ``erased`.
+    
+   It says that that Spec effect is idempotent and non-dependent,
+   meaning that if evaluating `f` on an argument `v:a`, exhibits an
+   effect `Spec` and returns a result; then the effect does not depend
+   on `v` and it can be subsumed to exhibiting the effect first and
+   then computing `f v` purely.
+   
+   In other words, it "pulls" the effect out of `f`.
+
+   pull is useful to mimic a kind of Tot/Spec effect polymorphism. 
+   
+   E.g.,  if you have `f: a -> Spec b` and a `l:list a`
+          you can do List.map (pull f) l : Spec (list b)
+ *)
+val pull (#a #b:Type) (f: a -> Spec b) : Spec (g:(a -> b) { forall x. f x == g x })
+
 /// The rest of this module includes several well-defined defined
 /// notions. They are not trusted.
 
@@ -80,7 +105,8 @@ let (let@) (x:erased 'a) (f:('a -> Tot (erased 'b))) : Tot (erased 'b) = bind x 
 (** Unary map *)
 irreducible
 let elift1 (#a #b: Type) (f: (a -> GTot b)) (x: erased a)
-    : Tot (y: erased b {reveal y == f (reveal x)}) = let@ xx = x in return (f xx)
+    : Tot (y: erased b {reveal y == f (reveal x)}) =
+  let@ xx = x in return (f xx)
 
 (** Binary map *)
 irreducible
